added typing rules

TAL.v
@@ -62,16 +62,16 @@ Inductive st : Type :=
 | St : heaps -> registers -> instr -> st.
 
 
-Inductive ieval : instr -> st -> st -> Prop :=
-| R_IAss : forall H R I d a1 pf, ieval (IAss d pf a1) (St H R (ISeq (IAss d pf a1) I)) (St H (t_update R (Id d) (aeval a1 R)) I)
-| R_IAdd : forall H R I d s pf1 pf2, ieval (IAdd d s pf1 pf2) (St H R (ISeq (IAdd d s pf1 pf2) I)) (St H (t_update R (Id s) (aeval (AReg d) R + aeval (AReg s) R)) I)
-| R_ISub : forall H R I d v pf1, ieval (ISub d v pf1) (St H R (ISeq (ISub d v pf1) I)) (St H (t_update R (Id d) (aeval (AReg d) R - aeval (ANum v) R)) I)
-| R_IJmp_Succ : forall H R I' v, H (Id v) = Some I' -> ieval (IJmp (ANum v)) (St H R (IJmp (ANum v))) (St H R I')
-| R_IJmp_Fail : forall H R I v, H (Id v) = None -> ieval I (St H R I) (St H R I)
-| R_IIf_EQ : forall H R I I' v r pf, aeval (AReg r) R = 0 -> (H (Id (R (Id v)))) = Some I' -> ieval (IIf r pf (AReg v)) (St H R I) (St H R I')
-| R_IIf_NEQ : forall H R I v r pf, aeval (AReg r) R <> 0 -> ieval (IIf r pf (AReg v)) (St H R (ISeq (IIf r pf (AReg v)) I)) (St H R I)   
-| R_ISeq : forall st st' st'' i1 i2, ieval i1 st st' -> ieval i2 st' st'' -> ieval (ISeq i1 i2) st st''
-| R_IStuck : forall st i, ieval i st st
+Inductive ieval : st -> st -> Prop :=
+| R_IAss : forall H R I d a1 pf, ieval (St H R (ISeq (IAss d pf a1) I)) (St H (t_update R (Id d) (aeval a1 R)) I)
+| R_IAdd : forall H R I d s pf1 pf2, ieval (St H R (ISeq (IAdd d s pf1 pf2) I)) (St H (t_update R (Id s) (aeval (AReg d) R + aeval (AReg s) R)) I)
+| R_ISub : forall H R I d v pf1, ieval (St H R (ISeq (ISub d v pf1) I)) (St H (t_update R (Id d) (aeval (AReg d) R - aeval (ANum v) R)) I)
+| R_IJmp_Succ : forall H R I v, H (Id (R (Id v))) = Some I -> ieval (St H R (IJmp (ANum v))) (St H R I)
+| R_IJmp_Fail : forall H R I v, H (Id (R (Id v))) = None -> ieval (St H R I) (St H R I)
+| R_IIf_EQ : forall H R I I' v r, aeval (AReg r) R = 0 -> (H (Id (R (Id v)))) = Some I' -> ieval (St H R I) (St H R I')
+| R_IIf_NEQ : forall H R I v r pf, aeval (AReg r) R <> 0 -> ieval (St H R (ISeq (IIf r pf (AReg v)) I)) (St H R I)   
+| R_ISeq : forall st st' st'', ieval st st' -> ieval st' st'' -> ieval st st''
+| R_IStuck : forall st, ieval st st
 .
 
 Definition threeLEten := (lt_n_S 2 9 (lt_n_S 1 8 (lt_n_S 0 7 (lt_0_Sn 6)))).
@@ -82,21 +82,70 @@ Definition oneLEten :=  (lt_n_S 0 9 (lt_0_Sn 8)).
 
 Definition init_heap := (update (update (update empty_heap (Id 1) (ISeq (IAss 3 threeLEten (ANum 0)) (IJmp (ANum 2)))) (Id 2) (ISeq (IIf 1 oneLEten (ANum 3)) (ISeq (IAdd 2 3 twoLEten threeLEten) (ISeq (ISub 1 1 oneLEten) (IJmp (ANum 2))) ))  )  (Id 3) (IJmp (AReg 4)) ).
 
-Definition init_regs :=  (t_update (t_update empty_regs (Id 1) 1) (Id 2) 2).
-Definition final_regs := (t_update (t_update (t_update empty_regs (Id 1) 0) (Id 2) 2) (Id 3) 2).
+Definition init_regs : registers :=  (t_update (t_update  (t_update (t_update (t_update empty_regs (Id 5) 1) (Id 6) 2) (Id 7) 3) (Id 1) 1) (Id 2) 2).
+Definition final_regs : registers := (t_update (t_update (t_update  (t_update (t_update (t_update empty_regs (Id 5) 1) (Id 6) 2) (Id 7) 3) (Id 1) 0) (Id 2) 2) (Id 3) 2).
 
-Eval compute in init_heap (Id 2).
+Eval compute in init_heap (Id (init_regs (Id 6))).
 
-(* find product of numbers stored in R1 and R2, store in R3
-*)
-(*Example ieval_example1 : ieval (ISeq (IAss 3 threeLEten (ANum 0)) (IJmp (ANum 2))) (St init_heap init_regs (ISeq (IAss 3 threeLEten (ANum 0)) (IJmp (ANum 2)))) ((St init_heap final_regs (IJmp (ANum 4)))).
+(* find product of numbers stored in R1 and R2, store in R3 
+
+Example ieval_example1 : ieval (St init_heap init_regs (ISeq (IAss 3 threeLEten (ANum 0)) (IJmp (ANum 2)))) ((St init_heap final_regs (IJmp (ANum 4)))).
 Proof.
   apply R_ISeq with (St init_heap (t_update init_regs (Id 3) 0) (IJmp (ANum 2))).
   apply R_IAss.
   apply R_IJmp_Succ with (St init_heap (t_update init_regs (Id 3) 0)
                           (ISeq (IIf 1 oneLEten (ANum 3))
                           (ISeq (IAdd 2 3 twoLEten threeLEten)
-                                (ISeq (ISub 1 1 oneLEten) (IJmp (ANum 2)))))).
+                          (ISeq (ISub 1 1 oneLEten) (IJmp (ANum 2)))))).
   
   simpl.
- *)
+*)
+
+Inductive ty : Type :=
+| int : ty
+| code : partial_map ty -> ty
+| arrow : partial_map ty -> partial_map ty -> ty                           
+| True : ty.
+
+
+Definition context := partial_map ty.
+
+(* register file types *)
+Definition Gamma : context := empty.
+
+(* instruction types *)
+Definition Psi : context := empty.
+
+(* typing rules for arithmetic expressions *)
+Inductive ahas_type : context -> context -> aexp -> ty -> Prop :=
+| S_Reg : forall Psi Gamma (r : nat) tau, r < K -> Gamma (Id r) = Some tau -> ahas_type Psi Gamma (AReg r) tau 
+| S_Int : forall Psi Gamma (n : nat), ahas_type Psi Gamma (ANum n) int.
+
+Hint Constructors ahas_type.
+
+Inductive ihas_type : context -> context -> instr -> ty -> Prop :=
+| S_Mov : forall Psi Gamma v tau d pf, ahas_type Psi Gamma v tau -> ihas_type Psi (update Gamma (Id d) tau) (IAss d pf v) tau
+| S_Add : forall Psi Gamma s d pf1 pf2, ahas_type Psi Gamma (AReg s) int -> ahas_type Psi Gamma (AReg d) int -> ihas_type Psi Gamma (IAdd d s pf1 pf2) int
+| S_If :  forall Psi Gamma s v pf1, ahas_type Psi Gamma (AReg s) int -> ahas_type Psi Gamma (AReg v) (code Gamma) -> ihas_type Psi Gamma (IIf s pf1 (AReg v)) (arrow Gamma Gamma)
+| S_Jump :  forall Psi Gamma v,  ahas_type Psi Gamma (AReg v) (code Gamma) -> ihas_type Psi Gamma (IJmp (AReg v)) (code Gamma)
+| S_Seq :  forall Psi i1 i2 Gamma Gamma2,  ihas_type Psi Gamma i1 (arrow Gamma Gamma2) -> ihas_type Psi Gamma i2 (code Gamma2) -> ihas_type Psi Gamma (ISeq i1 i2) (code Gamma).
+
+Hint Constructors ihas_type.
+
+
+Inductive Rhas_type : context -> registers -> context -> Prop :=
+| S_Regfile : forall r Psi Gamma (R : registers) tau, r < K ->  (Gamma (Id r)) = Some tau -> ahas_type Psi Gamma (AReg r) tau -> Rhas_type Psi R Gamma.
+
+Hint Constructors Rhas_type.
+
+Inductive Hhas_type : heaps -> context -> Prop :=
+  | S_Heap : forall Psi Gamma (H : heaps) l tau i, Psi (Id l) = Some tau -> H (Id l) = Some i -> ihas_type Psi Gamma i tau -> Hhas_type H Psi.
+
+Hint Constructors Hhas_type.
+
+Inductive M_ok : heaps -> registers -> instr -> Prop :=
+| S_Mach : forall H R I Psi Gamma , Hhas_type H Psi -> Rhas_type Psi R Gamma -> ihas_type Psi Gamma I (code Gamma) -> M_ok H R I.
+
+Hint Constructors M_ok.
+
+                                           
